nested hyper heaps

lib/hyperheap2.fsi
@@ -20,88 +20,48 @@
 module HyperHeap
 open Map
 open Heap
-type rid = list int
+type rid
 type t = Map.t rid heap
 new_effect STATE = STATE_h t
-opaque val root : rid
-let root = []
-
-private type rref (id:rid) (a:Type) = Prims.ref a
-val as_ref : #a:Type -> #id:rid -> r:rref id a -> Tot (ref a)
-let as_ref id r = r
-
-private val ref_as_rref : #a:Type -> i:rid -> r:ref a -> Tot (rref i a)
-let ref_as_rref i r = r
-
+val root : rid
+type rref : rid -> Type -> Type
+val as_ref      : #a:Type -> #id:rid -> r:rref id a -> GTot (ref a)
+val ref_as_rref : #a:Type -> i:rid -> r:ref a -> GTot (rref i a)
 val lemma_as_ref_inj: #a:Type -> #i:rid -> r:rref i a
     -> Lemma (requires (True))
              (ensures ((ref_as_rref i (as_ref r) = r)))
        [SMTPat (as_ref r)]
-let lemma_as_ref_inj i r = ()
 
 effect ST (a:Type) (pre:t -> Type) (post:t -> a -> t -> Type) =
        STATE a (fun 'p m0 -> pre m0 /\ (forall x m1. post m0 x m1 ==> 'p x m1))
                (fun 'p m0 ->  (forall x m1. pre m0 /\ post m0 x m1 ==> 'p x m1))
 
 val includes : rid -> rid -> Tot bool
-let rec includes r1 r2 =
-  if r1=r2 then true
-  else if List.length r2 > List.length r1
-  then includes r1 (Cons.tl r2)
-  else false
-
-let disjoint (i:rid) (j:rid) =
-  not (includes i j) && not (includes j i)
-
-private val lemma_aux: k:rid -> i:rid
-      -> Lemma  (requires
-                    List.length k > 0
-                    /\ List.length k <= List.length i
-                    /\ includes k i
-                    /\ not (includes (Cons.tl k) i))
-                 (ensures False)
-                 (decreases (List.length i))
-let rec lemma_aux k i = lemma_aux k (Cons.tl i)
-
-val lemma_disjoint_includes: i:rid -> j:rid -> k:rid ->
-  Lemma (requires (disjoint i j /\ includes j k))
-        (ensures (disjoint i k))
-        (decreases (List.length k))
-        [SMTPat (disjoint i j);
-         SMTPat (includes j k)]
-let rec lemma_disjoint_includes i j k =
-  if List.length k <= List.length j
-  then ()
-  else (lemma_disjoint_includes i j (Cons.tl k);
-        if List.length i <= List.length (Cons.tl k)
-        then ()
-        else (if includes k i
-              then lemma_aux k i
-              else ()))
-
-val extends: rid -> rid -> Tot bool
-let extends r0 r1 = is_Cons r0 && Cons.tl r0 = r1
+val extends  : rid -> rid -> Tot bool
+let disjoint i j = not (includes i j) && not (includes j i)
 
 val lemma_includes_refl: i:rid
                       -> Lemma (requires (True))
                                (ensures (includes i i))
                                [SMTPat (includes i i)]
-let lemma_includes refl i = ()
-  
+
+val lemma_disjoint_includes: i:rid -> j:rid -> k:rid ->
+  Lemma (requires (disjoint i j /\ includes j k))
+        (ensures (disjoint i k))
+        [SMTPat (disjoint i j);
+         SMTPat (includes j k)]
+
 val lemma_extends_includes: i:rid -> j:rid ->
-  Lemma (requires (extends j i))
-        (ensures (includes i j))
-        [SMTPat (extends j i)]
-let lemma_extends_includes i j = ()
+ Lemma (requires (extends j i))
+       (ensures (includes i j))
+       [SMTPat (extends j i)]
 
 val lemma_extends_disjoint: i:rid -> j:rid -> k:rid ->
-    Lemma (requires (extends j i /\ extends k i /\ j<>k))
-          (ensures (disjoint j k))
-let lemma_extends_disjoint i j k = ()
-
-let test0 = assert (includes [1;0] [2;1;0])
-let test1 (r1:rid) (r2:rid{includes r1 r2}) = assert (includes r1 (0::r2))
-
+   Lemma (requires (extends j i /\ extends k i /\ j<>k))
+         (ensures (disjoint j k))
+         [SMTPat (extends j i);
+          SMTPat (extends k i)]
+            
 type fresh_region (i:rid) (m0:t) (m1:t) =
  (forall j. includes i j ==> not (Map.contains m0 j))
  /\ Map.contains m1 i
@@ -109,33 +69,33 @@ type fresh_region (i:rid) (m0:t) (m1:t) =
 let sel (#a:Type) (#i:rid) (m:t) (r:rref i a) = Heap.sel (Map.sel m i) (as_ref r)
 let upd (#a:Type) (#i:rid) (m:t) (r:rref i a) (v:a) = Map.upd m i (Heap.upd (Map.sel m i) (as_ref r) v)
 
-assume val new_region: r0:rid -> ST rid
+val new_region: r0:rid -> ST rid
       (requires (fun m -> True))
       (ensures (fun (m0:t) (r1:rid) (m1:t) ->
                            extends r1 r0
                         /\ fresh_region r1 m0 m1
                         /\ m1=Map.upd m0 r1 Heap.emp))
 
-assume val ralloc: #a:Type -> i:rid -> init:a -> ST (rref i a)
+val ralloc: #a:Type -> i:rid -> init:a -> ST (rref i a)
     (requires (fun m -> True))
     (ensures (fun m0 x m1 ->
                     Let (Map.sel m0 i) (fun region_i ->
                     not (Heap.contains region_i (as_ref x))
                     /\ m1=Map.upd m0 i (Heap.upd region_i (as_ref x) init))))
 
-assume val op_Colon_Equals: #a:Type -> #i:rid -> r:rref i a -> v:a -> ST unit
+val op_Colon_Equals: #a:Type -> #i:rid -> r:rref i a -> v:a -> ST unit
   (requires (fun m -> True))
   (ensures (fun m0 _u m1 -> m1=Map.upd m0 i (Heap.upd (Map.sel m0 i) (as_ref r) v)))
 
-assume val op_Bang:#a:Type -> #i:rid -> r:rref i a -> ST a
+val op_Bang:#a:Type -> #i:rid -> r:rref i a -> ST a
   (requires (fun m -> True))
   (ensures (fun m0 x m1 -> m1=m0 /\ x=Heap.sel (Map.sel m0 i) (as_ref r)))
 
-assume val get: unit -> ST t
+val get: unit -> ST t
   (requires (fun m -> True))
   (ensures (fun m0 x m1 -> m0=x /\ m1=m0))
 
-assume val mod_set : Set.set rid -> Tot (Set.set rid)
+val mod_set : Set.set rid -> Tot (Set.set rid)
 assume Mod_set_def: forall (x:rid) (s:Set.set rid). {:pattern Set.mem x (mod_set s)}
                     Set.mem x (mod_set s) <==> (exists (y:rid). Set.mem y s /\ includes y x)
 
@@ -146,7 +106,6 @@ val lemma_modifies_trans: m1:t -> m2:t -> m3:t
                        -> s1:Set.set rid -> s2:Set.set rid
                        -> Lemma (requires (modifies s1 m1 m2 /\ modifies s2 m2 m3))
                                 (ensures (modifies (Set.union s1 s2) m1 m3))
-let lemma_modifies_trans m1 m2 m3 s1 s2 = ()
 
 type contains_ref (#a:Type) (#i:rid) (r:rref i a) (m:t) =
     Map.contains m i /\ Heap.contains (Map.sel m i) (as_ref r)
