doc/tutorial/code/solutions/robot2.fst
@@ -1,10 +1,11 @@
 (*--build-config
-    options:--admit_fsi Set --admit_fsi Map --z3timeout 20;
+    options:--admit_fsi Set --admit_fsi Map --admit_fsi HyperHeap --max_fuel 0 --initial_ifuel 0;
     variables:LIB=../../../../lib;
-    other-files:$LIB/ext.fst $LIB/set.fsi $LIB/heap.fst $LIB/map.fsi $LIB/list.fst $LIB/hyperheap2.fst
+    other-files:$LIB/ext.fst $LIB/set.fsi $LIB/heap.fst $LIB/map.fsi $LIB/hyperheap2.fsi $LIB/util.fst
 --*)
 module Robot
-open List
+#set-options "--initial_fuel 0 --max_ifuel 0"
+open Util
 open Heap
 open HyperHeap
 
@@ -21,9 +22,6 @@ type arm =
        -> azim:rref r int{polar <> azim}
        -> arm
 
-let disjoint (i:rid) (j:rid) =
-  not (includes i j) && not (includes j i)
-
 type bot =
   | Bot : #r:rid
        -> pos  :point{includes r (Point.r pos)}
@@ -33,48 +31,6 @@ type bot =
                         /\ disjoint (Point.r pos) (Arm.r right)
                         /\ disjoint (Arm.r left)  (Arm.r right)}
        -> bot
-
-let refs_in_point (p:point) =
-  !{as_ref (Point.x p),
-    as_ref (Point.y p),
-    as_ref (Point.z p)}
-
-let refs_in_arm (a:arm) =
-  !{as_ref (Arm.polar a),
-    as_ref (Arm.azim a)}
-
-let op_Plus_Plus x y = Set.union x y
-let op_Plus_Plus_Hat x y = x ++ (Set.singleton y)
-let op_Hat_Plus_Hat  x y = (Set.singleton x) ++ (Set.singleton y)
-
-let refs (b:bot) =
-  refs_in_point (Bot.pos b)
-  ++ refs_in_arm (Bot.left b)
-  ++ refs_in_arm (Bot.right b)
-
-let regions (b:bot) =
-  Bot.r b
-  ^+^ Point.r (Bot.pos b)
-  ++^ Arm.r (Bot.left  b)
-  ++^ Arm.r (Bot.right b)
-
-  (*/\ (forall (a:Type) (r:ref a). Set.mem (Heap.Ref r) (refs b)
-                ==> Heap.contains (Map.sel h (Robot.i x)) r)*)
-
-opaque type modifies1 (s:Set.set rid) (m0:t) (m1:t) =
-  (forall (id:rid). Map.contains m0 id ==> Map.contains m1 id)
-  /\ (forall (id:rid).//{:pattern (Map.sel m1 id)}
-            Map.contains m0 id
-            /\ (forall (mod:rid). Set.mem mod s ==> not (includes mod id))
-            ==> Map.sel m1 id = Map.sel m0 id)
-
-assume val mod_set : Set.set rid -> Tot (Set.set rid)
-assume Mod_set_def: forall (x:rid) (s:Set.set rid). {:pattern Set.mem x (mod_set s)}
-                    Set.mem x (mod_set s) <==> (exists (y:rid). Set.mem y s /\ includes y x)
-
-
-opaque logic type modifies (s:Set.set rid) (m0:t) (m1:t) =
-  Map.Equal m1 (Map.concat m1 (Map.restrict (Set.complement (mod_set s)) m0))
 
 let flying (b:bot) (h:HyperHeap.t) =
     sel h (Point.z (Bot.pos b)) > 0
@@ -90,22 +46,10 @@ type robot_inv (b:bot) (h:HyperHeap.t) =
   /\ Map.contains h (Arm.r (Bot.right b))
   /\ (flying b h ==> arms_up b h)
 
-assume val lemma_disjoint_includes: i:rid -> j:rid -> k:rid ->
-  Lemma (requires (disjoint i j /\ includes j k))
-        (ensures (disjoint i k))
-        [SMTPat (disjoint i j);
-         SMTPat (includes j k)]
-(*let lemma_disjoint_includes i j k = ()*)
-
-assume val lemma_modifies_trans: m1:HyperHeap.t -> m2:HyperHeap.t -> m3:HyperHeap.t
-                        -> s1:Set.set rid -> s2:Set.set rid
-                        -> Lemma (requires (modifies s1 m1 m2 /\ modifies s2 m2 m3))
-                                 (ensures (modifies (Set.union s1 s2) m1 m3))
-                                 (*[SMTPatT (modifies s1 m1 m2);
-                                  SMTPatT (modifies s2 m2 m3)]*)
+let only i = Set.singleton i
 
 val lemma_frame_robot_inv1 : b:bot -> h0:HyperHeap.t -> h1:HyperHeap.t -> i:rid{disjoint i (Bot.r b)}
-  -> Lemma (requires (robot_inv b h0 /\ modifies (Set.singleton i) h0 h1))
+  -> Lemma (requires (robot_inv b h0 /\ modifies (only i) h0 h1))
            (ensures (robot_inv b h1))
 let lemma_frame_robot_inv1 b h0 h1 i = ()
 
@@ -162,7 +106,6 @@ let test1 r0 =
   admitP (modifies Set.empty m0 m1);
   assert (sel m1 x = 0)
 
-
 val new_robot: r0:rid -> ST bot (requires (fun h0 -> True))
                                 (ensures (fun h0 x h1 ->
                                       modifies Set.empty h0 h1
@@ -179,25 +122,25 @@ let new_robot r0 =
 val walk_robot_to: x:int -> y:int -> b:bot -> ST unit
     (requires (robot_inv b))
     (ensures (fun h0 u h1 ->
-                modifies (Set.singleton (Point.r (Bot.pos b))) h0 h1
+                modifies (only (Point.r (Bot.pos b))) h0 h1
                 /\ robot_inv b h1
                 /\ sel h1 (Point.z (Bot.pos b))  = sel h1 (Point.z (Bot.pos b))
                 /\ sel h1 (Point.x (Bot.pos b))  = x
                 /\ sel h1 (Point.y (Bot.pos b))  = y))
 let walk_robot_to x y b =
- op_ColonEquals (Point.x (Bot.pos b)) x;
- op_ColonEquals (Point.y (Bot.pos b)) y
+  Point.x (Bot.pos b) := x;
+  Point.y (Bot.pos b) := y
 
 val fly: b:bot -> ST unit
   (requires (robot_inv b))
   (ensures (fun h0 _u h1 ->
-              modifies (Set.singleton (Bot.r b)) h0 h1
+              modifies (only (Bot.r b)) h0 h1
               /\ robot_inv b h1
               /\ flying b h1))
 let fly b =
-  op_ColonEquals (Arm.polar (Bot.left b)) 0;
-  op_ColonEquals (Arm.polar (Bot.right b)) 0;
-  op_ColonEquals (Point.z (Bot.pos b)) 100
+  Arm.polar (Bot.left b)  := 0;
+  Arm.polar (Bot.right b) := 0;
+  Point.z (Bot.pos b)     := 100
 
 val fly_robots: b0:bot
              -> b1:bot{disjoint (Bot.r b0) (Bot.r b1)}
@@ -210,18 +153,13 @@ val fly_robots: b0:bot
               /\ flying b0 h1
               /\ flying b1 h1))
 let fly_robots b0 b1 =
-    let m0 = get () in
   fly b0;
-    let m1 = get () in
-  fly b1;
-    let m2 = get () in
-    lemma_frame_robot_inv1 b0 m1 m2 (Bot.r b1);
-    lemma_modifies_trans m0 m1 m2 (Set.singleton (Bot.r b0)) (Set.singleton (Bot.r b1))
+  fly b1
 
 val main: unit -> ST unit
     (requires (fun _ -> True))
     (ensures (fun m0 _ m1 -> modifies Set.empty m0 m1))
 let main () =
-  let b1 = new_robot [] in
-  let b2 = new_robot [] in
+  let b1 = new_robot root in
+  let b2 = new_robot root in
   fly_robots b1 b2
