lib/util.fst
@@ -1,0 +1,15 @@
+(*--build-config
+    options:--admit_fsi Heap --admit_fsi Heap --admit_fsi HyperHeap;
+    other-files:ext.fst set.fsi heap.fst map.fsi hyperheap2.fsi
+  --*)
+module Util
+
+let op_Plus_Plus x y = Set.union x y
+let op_Plus_Plus_Hat x y = x ++ (Set.singleton y)
+let op_Hat_Plus_Hat  x y = (Set.singleton x) ++ (Set.singleton y)
+
+open Heap
+open HyperHeap
+let op_At_Plus_At (#a:Type) (#r:rid) (#b:Type) (#s:rid) (x:rref r a) (y:rref s b) =
+   Ref (as_ref x) ^+^ Ref (as_ref y)
+let op_Plus_Plus_At (#a:Type) (#r:rid) (x:Set.set aref) (y:rref r a) = x ++^ Ref (as_ref y)
